src/RenamingEquations.v
@@ -2,7 +2,7 @@ Require Import String PeanoNat Compare_dec
         StrictProp Setoid Morphisms.
 Require Import Morph Var VarEquations Renaming.
 
-(* Properties of composition *)
+(* Properties of closing composition *)
 
 Definition apply_closing_rhs_var {N M} (r : closing_rhs N M)
   : morph var M var (S N) :=
@@ -18,88 +18,95 @@ Definition apply_closing_rhs_var {N M} (r : closing_rhs N M)
       @ morph_extend_by M (@close_var n)
   end.
 
-Lemma apply_closing_rhs_weak N M
-      (l : level N) (r : closing_rhs (pred N) M) :
-  apply_closing_rhs_var (closing_rhs_weak l r)
-  =m= lift_morph_var (@cycle_out_var N l)
-      @ lift_morph_var (morph_id_from_succ_pred l)
-      @ morph_extend_by (pred N) (@swap_var)
+Lemma apply_closing_rhs_zero_weak N M
+      (r : closing_rhs N M) :
+  apply_closing_rhs_var (closing_rhs_zero_weak r)
+  =m= morph_extend_by N (@swap_var)
       @ lift_morph_var (apply_closing_rhs_var r)
       @ morph_extend_by M (@weak_var).
 Proof.
   destruct r; cbn.
-  - inversion_level l.
-    simplify_var_morphs.
+  - simplify_var_morphs.
     setoid_rewrite transpose_swap_lifted'.
     transpose_pushes weak_op weak_op at 1.
     easy.
-  - inversion_level l.
-    simplify_var_morphs.
+  - simplify_var_morphs.
     setoid_rewrite transpose_swap_lifted'.
-    transpose_pushes weak_op (cycle_in_op l0).
+    transpose_pushes weak_op (cycle_in_op l).
     easy.
-  - inversion_level l.
-    simplify_var_morphs.
+  - simplify_var_morphs.
     setoid_rewrite transpose_swap_lifted'.
     transpose_pushes weak_op (close_op n).
     easy.
 Qed.
 
-Lemma apply_closing_rhs_exchange N M
-      (l1 : level N) (r : closing_rhs (pred N) M)
-      (l2 : level (S M)):
-  apply_closing_rhs_var (closing_rhs_exchange l1 r l2)
-  =m= lift_morph_var (@cycle_out_var N l1)
-      @ lift_morph_var (morph_id_from_succ_pred l1)
-      @ morph_extend_by (pred N) (@swap_var)
+Lemma apply_closing_rhs_zero_exchange N M
+      (r : closing_rhs N M) (l2 : level (S M)):
+  apply_closing_rhs_var (closing_rhs_zero_exchange r l2)
+  =m= morph_extend_by N (@swap_var)
       @ lift_morph_var (apply_closing_rhs_var r)
       @ (@cycle_in_var (S M) l2).
 Proof.
   destruct r; cbn.
-  - inversion_level l1.
-    simplify_var_morphs.
+  - simplify_var_morphs.
     setoid_rewrite transpose_swap_lifted'.
     transpose_pushes (cycle_in_op l2) weak_op.
     easy.
-  - inversion_level l1.
-    simplify_var_morphs.
+  - simplify_var_morphs.
     setoid_rewrite transpose_swap_lifted'.
     transpose_pushes (cycle_in_op l) (cycle_in_op l2).
     rewrite swap_swap_identity'.
     easy.
-  - inversion_level l1.
-    simplify_var_morphs.
+  - simplify_var_morphs.
     setoid_rewrite transpose_swap_lifted'.
     transpose_pushes (cycle_in_op l2) (close_op n).
     easy.
 Qed.
 
-Lemma apply_closing_rhs_close N M
-      (l : level N) (r : closing_rhs (pred N) M) n :
-  apply_closing_rhs_var (closing_rhs_close l r n)
-  =m= lift_morph_var (@cycle_out_var N l)
-      @ lift_morph_var (morph_id_from_succ_pred l)
-      @ morph_extend_by (pred N) (@swap_var)
+Lemma apply_closing_rhs_zero_close N M
+      (r : closing_rhs N M) n :
+  apply_closing_rhs_var (closing_rhs_zero_close r n)
+  =m= morph_extend_by N (@swap_var)
       @ lift_morph_var (apply_closing_rhs_var r)
       @ morph_extend_by M (@close_var n).
 Proof.
   destruct r; cbn.
-  - inversion_level l.
-    simplify_var_morphs.
+  - simplify_var_morphs.
     setoid_rewrite transpose_swap_lifted'.
     transpose_pushes (close_op n) weak_op.
     easy.
-  - inversion_level l.
-    simplify_var_morphs.
+  - simplify_var_morphs.
     setoid_rewrite transpose_swap_lifted'.
-    transpose_pushes (close_op n) (cycle_in_op l0).
+    transpose_pushes (close_op n) (cycle_in_op l).
     easy.
-  - inversion_level l.
-    simplify_var_morphs.
+  - simplify_var_morphs.
     setoid_rewrite transpose_swap_lifted'.
     transpose_pushes (close_op _) (close_op n).
     rewrite swap_swap_identity'.
     easy.
+Qed.
+
+Definition apply_closing_var_with_cycle_out {N M}
+           (r : closing N M) : morph var M var N :=
+  match r in closing N M return morph var M var N with
+  | closing_nil =>
+    apply_closing_var closing_nil
+  | closing_zero_weak r =>
+    (@cycle_out_var _ l_0)
+    @ apply_closing_var (closing_zero_weak r)
+  | closing_zero_exchange r l =>
+    (@cycle_out_var _ l_0)
+    @ apply_closing_var (closing_zero_exchange r l)
+  | closing_zero_close r n =>
+    (@cycle_out_var _ l_0)
+    @ apply_closing_var (closing_zero_close r n)
+  end.
+
+Lemma apply_closing_var_add_cycle_out {N M} (r : closing N M) :
+  apply_closing_var r =m= apply_closing_var_with_cycle_out r.
+Proof.
+  induction r; cbn;
+    try rewrite cycle_out_zero_identity; simplify_var_morphs; easy.
 Qed.
 
 Lemma apply_transpose_level_closing_aux N M
@@ -111,42 +118,47 @@ Lemma apply_transpose_level_closing_aux N M
   apply_closing_rhs_var (transpose_level_closing r l).
 Proof.
   generalize dependent l.
-  induction r; intro l'; cbn; try rewrite morph_left_identity.
+  induction r; intro l'; rewrite apply_closing_var_add_cycle_out;
+    cbn; try rewrite morph_left_identity.
   - exfalso; apply (level_zero_empty l').
   - unfold level_sdec.
-    destruct (level_dec l' l); subst; cbn.
+    destruct (level_dec l_0 l'); subst; cbn.
     + rewrite morph_associative.
       rewrite cycle_in_cycle_out_identity.
-      rewrite morph_left_identity.
       easy.
-    + inversion_level (unshift_level_neq l' l (squash n)).
-      rewrite apply_closing_rhs_weak; cbn.
+    + inversion_level (unshift_level_neq l_0 l' (squash n)).
+      rewrite morph_associative.
+      transpose_push_pop (cycle_in_op l') (cycle_out_op l_0).
+      rewrite cycle_out_zero_identity.
+      rewrite apply_closing_rhs_zero_weak; cbn.
       rewrite <- IHr; cbn.
       simplify_var_morphs.
-      rewrite morph_associative.
-      transpose_push_pop (cycle_in_op l') (cycle_out_op l).
       easy.
   - unfold level_sdec.
-    destruct (level_dec l' l); subst; cbn.
-    + rewrite cycle_in_cycle_out_identity'.
+    destruct (level_dec l_0 l'); subst; cbn.
+    + rewrite morph_associative.
+      rewrite cycle_in_cycle_out_identity.
       easy.
-    + inversion_level (unshift_level_neq l' l (squash n)).
-      rewrite apply_closing_rhs_exchange; cbn.
+    + inversion_level (unshift_level_neq l_0 l' (squash n)).
+      rewrite morph_associative.
+      transpose_push_pop (cycle_in_op l') (cycle_out_op l_0).
+      rewrite cycle_out_zero_identity.
+      rewrite apply_closing_rhs_zero_exchange; cbn.
       rewrite <- IHr; cbn.
       simplify_var_morphs.
-      rewrite morph_associative.
-      transpose_push_pop (cycle_in_op l') (cycle_out_op l).
       easy.
   - unfold level_sdec.
-    destruct (level_dec l' l); subst; cbn.
-    + rewrite cycle_in_cycle_out_identity'.
+    destruct (level_dec l_0 l'); subst; cbn.
+    + rewrite morph_associative.
+      rewrite cycle_in_cycle_out_identity.
       easy.
-    + inversion_level (unshift_level_neq l' l (squash n0)).
-      rewrite apply_closing_rhs_close; cbn.
+    + inversion_level (unshift_level_neq l_0 l' (squash n0)).
+      rewrite morph_associative.
+      transpose_push_pop (cycle_in_op l') (cycle_out_op l_0).
+      rewrite cycle_out_zero_identity.
+      rewrite apply_closing_rhs_zero_close; cbn.
       rewrite <- IHr; cbn.
       simplify_var_morphs.
-      rewrite morph_associative.
-      transpose_push_pop (cycle_in_op l') (cycle_out_op l).
       easy.
 Qed.
 
@@ -156,7 +168,150 @@ Lemma apply_transpose_level_closing N M
   =m=
   apply_closing_rhs_var (transpose_level_closing r l).
 Proof.
-  rewrite <- apply_transpose_level_closing_aux; cbn.
-  rewrite morph_left_identity.
+  rewrite <- apply_transpose_level_closing_aux.
   easy.
+Qed.
+
+Lemma transpose_closing_weak {N M} (r : closing N M) :
+  lift_morph_var (apply_closing_var r)
+  @ morph_extend_by M (@weak_var)
+  =m= morph_extend_by N (@weak_var)
+      @ apply_closing_var r.
+Proof.
+  induction r; rewrite apply_closing_var_add_cycle_out;
+    cbn; simplify_var_morphs; try easy.
+  - rewrite morph_associative
+      with (g := @cycle_out_var _ _).
+    transpose_push_pop weak_op (cycle_out_op l_0).
+    simplify_var_morphs.
+    rewrite morph_associative
+      with (g := lift_morph_var (apply_closing_var r)).
+    rewrite <- lift_morph_var_compose.
+    rewrite <- IHr.
+    simplify_var_morphs.
+    rewrite morph_associative
+      with (f := morph_extend_by N (@swap_var)).
+    rewrite transpose_swap_lifted.
+    simplify_var_morphs.
+    transpose_pushes weak_op weak_op at 1.
+    easy.
+  - rewrite morph_associative with (g := @cycle_out_var _ l_0).
+    transpose_push_pop weak_op (cycle_out_op l_0).
+    transpose_pushes (cycle_in_op l) weak_op.
+    rewrite morph_associative
+      with (g := morph_extend_by M (@swap_var)).
+    rewrite <- transpose_swap_lifted.
+    simplify_var_morphs.
+    rewrite morph_associative
+      with (g := lift_morph_var (apply_closing_var r)).
+    rewrite <- lift_morph_var_compose.
+    rewrite <- IHr.
+    simplify_var_morphs.
+    easy.
+  - rewrite morph_associative with (g := @cycle_out_var _ l_0).
+    transpose_push_pop weak_op (cycle_out_op l_0).
+    transpose_pushes (close_op n) weak_op.
+    rewrite morph_associative
+      with (g := morph_extend_by M (@swap_var)).
+    rewrite <- transpose_swap_lifted.
+    simplify_var_morphs.
+    rewrite morph_associative
+      with (g := lift_morph_var (apply_closing_var r)).
+    rewrite <- lift_morph_var_compose.
+    rewrite <- IHr.
+    simplify_var_morphs.
+    easy.
+Qed.
+
+Lemma apply_transpose_name_closing N M
+      (r : closing N M) n:
+  morph_extend_by N (@close_var n) @ apply_closing_var r
+  =m=
+  apply_closing_rhs_var (transpose_name_closing r n).
+Proof.
+  induction r; rewrite apply_closing_var_add_cycle_out;
+    cbn; simplify_var_morphs; try easy.
+  - rewrite apply_closing_rhs_zero_weak, <- IHr;
+      cbn; simplify_var_morphs.
+    rewrite morph_associative with (g := @cycle_out_var _ l_0).
+    transpose_push_pop (close_op n) (cycle_out_op l_0).
+    rewrite cycle_out_zero_identity.
+    simplify_var_morphs.
+    easy.
+  - rewrite apply_closing_rhs_zero_exchange, <- IHr;
+      cbn; simplify_var_morphs.
+    rewrite morph_associative with (g := @cycle_out_var _ l_0).
+    transpose_push_pop (close_op n) (cycle_out_op l_0).
+    rewrite cycle_out_zero_identity.
+    simplify_var_morphs.
+    easy.
+  - rewrite apply_closing_rhs_zero_close, <- IHr;
+      cbn; simplify_var_morphs.
+    rewrite morph_associative with (g := @cycle_out_var _ l_0).
+    transpose_push_pop (close_op n) (cycle_out_op l_0).
+    rewrite cycle_out_zero_identity.
+    simplify_var_morphs.
+    easy.
+Qed.
+
+Lemma apply_compose_closing {N M O}
+    (r1 : closing O N) (r2 : closing N M) :
+  apply_closing_var (compose_closing r1 r2)
+  =m= apply_closing_var r1 @ apply_closing_var r2.
+Proof.
+  generalize dependent M.
+  induction r1; intros M' r2; cbn; try easy.
+  - rewrite IHr1; simplify_var_morphs.
+    setoid_rewrite transpose_closing_weak.
+    easy.
+  - simplify_var_morphs.
+    rewrite apply_transpose_level_closing.
+    destruct (transpose_level_closing r2 l); cbn;
+      rewrite IHr1; simplify_var_morphs; easy.
+  - simplify_var_morphs.
+    setoid_rewrite apply_transpose_name_closing.
+    destruct (transpose_name_closing r2 n); cbn;
+      rewrite IHr1; simplify_var_morphs; easy.
+Qed.
+
+Lemma transpose_level_id {N} (l : level (S N)) :
+  transpose_level_closing closing_id l
+  = closing_rhs_exchange_rhs closing_id l.
+Proof.
+  induction N; cbn in *; unfold level_sdec in *.
+  - destruct (level_dec l_0 l) as [eql|neql].
+    + rewrite eql; easy.
+    + exfalso.
+      apply (level_zero_empty
+               (unshift_level_neq l_0 l (squash neql))).
+  - destruct (level_dec l_0 l) as [eql|neql].
+    + rewrite eql; easy.
+    + rewrite IHN.
+      unfold closing_rhs_zero_exchange.
+      rewrite shift_level_unshift_level_neq_identity.
+      easy.
+Qed.
+
+Lemma transpose_name_id {N} n :
+  transpose_name_closing (@closing_id N) n
+  = closing_rhs_close_rhs closing_id n.
+Proof.
+  induction N; cbn; try rewrite IHN; easy.
+Qed.
+
+Lemma closing_left_identity {N M} (r : closing N M) :
+  compose_closing closing_id r = r.
+Proof.
+  induction r; cbn; try rewrite IHr; easy.
+Qed.
+
+Lemma closing_right_identity {N M} (r : closing N M) :
+  compose_closing r closing_id = r.
+Proof.
+  induction r; try easy.
+  - cbn; rewrite IHr; easy.
+  - remember (@closing_id (S M)) as c; cbn; subst.
+    rewrite transpose_level_id, IHr; easy.
+  - remember (@closing_id (S M)) as c; cbn; subst.
+    rewrite transpose_name_id, IHr; easy.
 Qed.
