src/Term.v
@@ -99,11 +99,11 @@ Module MakeTerm (T : Relative_monad).
       match v with
       | free n =>
         apply_closing
-          (closing_weak l0 closing_id_n) V (m V (free n))
-      | bound (mklevel 0 _) => unit (S N) (bound l0)
+          (closing_weak l_0 closing_id) V (m V (free n))
+      | bound (mklevel 0 _) => unit (S N) (bound l_0)
       | bound (mklevel (S l) lt) =>
         apply_closing
-          (closing_weak l0 closing_id_n) V
+          (closing_weak l_0 closing_id) V
           (m V (bound (mklevel l (less_than_pred lt))))
       end.
 
@@ -128,9 +128,13 @@ Module MakeTerm (T : Relative_monad).
   : morph term M term N :=
     kleisli (apply_substitution_k r).
 
-  Definition substitution_id : substitution term 0 0 :=
+  Definition substitution_nil : substitution term 0 0 :=
+    substitution_renaming (renaming_nil).
+  Arguments substitution_nil : simpl never.
+
+  Definition substitution_id {N} : substitution term N N :=
     substitution_renaming (renaming_id).
-  Arguments substitution_id : simpl never.
+  Arguments substitution_id {N} : simpl never.
 
   Fixpoint substitution_weak {N M}
            (l1 : level (S N)) (r : substitution term N M) :
@@ -142,13 +146,13 @@ Module MakeTerm (T : Relative_monad).
         substitution_bind
           (morph_apply_zero
              (apply_closing
-                (closing_weak l1 closing_id_n)) t)
+                (closing_weak l1 closing_id)) t)
           (substitution_weak l1 r) l
     | substitution_subst t r n =>
         substitution_subst
           (morph_apply_zero
              (apply_closing
-                (closing_weak l1 closing_id_n)) t)
+                (closing_weak l1 closing_id)) t)
           (substitution_weak l1 r) n
     end.
 
@@ -158,21 +162,22 @@ Module MakeTerm (T : Relative_monad).
     match r with
     | substitution_renaming r =>
       fun l2 =>
-        substitution_renaming (renaming_swap l1 r l2)
-    | substitution_bind t r l =>
+        substitution_renaming (renaming_exchange l1 r l2)
+    | @substitution_bind _ _ M' t r l =>
       fun l2 =>
         substitution_bind
           (morph_apply_zero
              (apply_closing
-                (closing_weak l1 closing_id_n)) t)
-          (substitution_swap l1 r (unshift_level l l2))
+                (closing_weak l1 closing_id)) t)
+          (substitution_swap l1 r
+             (@unshift_level (S (S M')) l l2))
           (shift_level l2 l)
     | substitution_subst t r n =>
       fun l2 =>
         substitution_subst
           (morph_apply_zero
              (apply_closing
-                (closing_weak l1 closing_id_n)) t)
+                (closing_weak l1 closing_id)) t)
           (substitution_swap l1 r l2) n
     end.
 
@@ -186,13 +191,13 @@ Module MakeTerm (T : Relative_monad).
         substitution_bind
           (morph_apply_zero
              (apply_closing
-                (closing_weak l closing_id_n)) t)
+                (closing_weak l closing_id)) t)
           (substitution_close l r n) l'
     | substitution_subst t r n' =>
         substitution_subst
           (morph_apply_zero
              (apply_closing
-                (closing_weak l closing_id_n)) t)
+                (closing_weak l closing_id)) t)
           (substitution_close l r (unshift_name n' n))
           (shift_name n n')
     end.
@@ -207,15 +212,13 @@ Module MakeTerm (T : Relative_monad).
         substitution_bind
           (morph_apply_zero
              (apply_renaming
-                (renaming_shift n
-                   renaming_id_n)) t)
+                (renaming_shift n renaming_id)) t)
           (substitution_shift n r) l
     | substitution_subst t r n' =>
         substitution_subst
           (morph_apply_zero
              (apply_renaming
-                (renaming_shift n
-                   renaming_id_n)) t)
+                (renaming_shift n renaming_id)) t)
           (substitution_shift n r) n'
     end.
 
@@ -226,22 +229,21 @@ Module MakeTerm (T : Relative_monad).
     | substitution_renaming r =>
       fun l =>
         substitution_renaming (renaming_open n r l)
-    | substitution_bind t r l' =>
+    | @substitution_bind _ _ M' t r l' =>
       fun l =>
         substitution_bind
           (morph_apply_zero
              (apply_renaming
-                (renaming_shift n
-                   renaming_id_n)) t)
-          (substitution_open n r (unshift_level l' l))
+                (renaming_shift n renaming_id)) t)
+          (substitution_open n r
+             (@unshift_level (S (S M')) l' l))
           (shift_level l l')
     | substitution_subst t r n' =>
       fun l =>
         substitution_subst
           (morph_apply_zero
              (apply_renaming
-                (renaming_shift n
-                   renaming_id_n)) t)
+                (renaming_shift n renaming_id)) t)
           (substitution_open n r l) n'
     end.
 
@@ -255,15 +257,13 @@ Module MakeTerm (T : Relative_monad).
         substitution_bind
           (morph_apply_zero
              (apply_renaming
-                (renaming_shift n1
-                   renaming_id_n)) t)
+                (renaming_shift n1 renaming_id)) t)
           (substitution_rename n1 r n2) l
     | substitution_subst t r n' =>
         substitution_subst
           (morph_apply_zero
              (apply_renaming
-                (renaming_shift n1
-                   renaming_id_n)) t)
+                (renaming_shift n1 renaming_id)) t)
           (substitution_rename n1 r (unshift_name n' n2))
           (shift_name n2 n')
     end.
@@ -326,952 +326,11 @@ Module MakeTerm (T : Relative_monad).
         n
     end.
 
-  Definition open_k n : morph var 1 term 0 :=
-    @unit 0 @ @open_var n.
-  Arguments open_k n {V} v /.
-
-  Definition open n := kleisli (@open_k n).
-  Arguments open n {V} t.
-
-  Definition close_k n : morph var 0 term 1 :=
-    @unit 1 @ @close_var n.
-  Arguments close_k n {V} v /.
-
-  Definition close n := kleisli (@close_k n).
-  Arguments close n {V} t.
-
-  Definition weak_k : morph var 0 term 1 :=
-    @unit 1 @ @weak_var.
-  Arguments weak_k {V} v /.
-
-  Definition weak := kleisli (@weak_k).
-  Arguments weak {V} t.
-
-  Fixpoint weaken (t : term 0) V : term (0 + V) :=
-    match V with
-    | 0 => t
-    | S V => @weak V (@weaken t V)
-    end.
-  Arguments weaken t {V}.
-
-  Definition bind_k t : morph var 1 term 0 :=
-    fun {V} v =>
-      match v with
-      | free n => unit 0 (free n)
-      | bound succ0 => weaken t
-      | bound (succS l) => unit 0 (bound l)
-      end.
-  Arguments bind_k t {V} v : simpl nomatch.
-
-  Definition bind t := kleisli (@bind_k t).
-  Arguments bind t {V} s.
-
   Add Parametric Morphism {N M} : (@kleisli N M)
     with signature eq_morph ==> eq_morph
     as kleisli_mor.
-    intros * Heq V n; unfold fst_ivar.
+    intros * Heq V n.
     apply extensional; easy.
   Qed.
 
-  (* [reducible r n] always equals [I], but this
-     is only true definitionally when [apply_renaming_k r (free n)]
-     is definitionally equal to a simpler expression.
-     This relies on the lack of definitional eta for [True]. *)
-  Fixpoint reducible (r : renaming term) {V} (v : var V)
-    : True :=
-      match r with
-      | r_id => I
-      | r_shift n r => reducible r v
-      | r_rename n1 r n2 =>
-          match v with
-          | bound _ => I
-          | free n =>
-            if name_dec n n2 then I
-            else @reducible r V (free (unshift_name n2 n))
-          end
-      | r_subst t r n1 =>
-          match v with
-          | bound _ => I
-          | free n =>
-            if name_dec n n1 then I
-            else @reducible r V (free (unshift_name n1 n))
-          end
-      end.
-
-  Fixpoint apply_renaming_k (r : renaming term)
-  : morph var 0 term 0 :=
-        fun V v =>
-          match reducible r v with
-          | I =>
-            match r with
-            | r_id => unit 0 v
-            | r_shift n r =>
-              open n (apply_renaming_k r (S V) (weak_var v))
-            | r_rename n1 r n2 =>
-              open n1 (apply_renaming_k r (S V) (close_var n2 v))
-            | r_subst t r n =>
-              bind t (apply_renaming_k r (S V) (close_var n v))
-            end
-          end.
-  Arguments apply_renaming_k r {V} v : simpl nomatch.
-
-  Definition apply_renaming r :=
-    kleisli (@apply_renaming_k r).
-  Arguments apply_renaming r {V} t.
-
-  Notation "[ r ] t" :=
-    (apply_renaming r%ren t)
-      (at level 65).
-
-  Fixpoint transpose_opens_open_left ns n :=
-    match ns with
-    | nil => n
-    | cons n2 ns =>
-      transpose_opens_open_left ns (shift_name n2 n)
-    end.
-
-  Fixpoint transpose_opens_bind_left ns (t : term 0) :=
-    match ns with
-    | nil => t
-    | cons n ns =>
-      transpose_opens_bind_left ns (open n (weak t))
-    end.
-
-  Fixpoint transpose_opens_renaming_open_left
-           ns (r : renaming term) n :=
-    match r with
-    | r_id => p_open (transpose_opens_open_left ns n)
-    | r_shift n2 r =>
-      transpose_opens_renaming_open_left (cons n2 ns) r n
-    | r_rename n2 r n3 =>
-      if name_dec n n3 then
-        p_open (transpose_opens_open_left ns n2)
-      else
-        transpose_opens_renaming_open_left
-          (cons n2 ns) r (unshift_name n3 n)
-    | r_subst t r n2 =>
-      if name_dec n n2 then
-        p_bind (transpose_opens_bind_left ns t)
-      else
-        transpose_opens_renaming_open_left ns r (unshift_name n2 n)
-    end.
-  Arguments transpose_opens_renaming_open_left ns r n
-    : simpl nomatch.
-
-  Definition transpose_open_pop_right (p : pop term) n :=
-    match p with
-    | p_open n2 => unshift_name n2 n
-    | p_bind _ => n
-    end.
-
-  Fixpoint transpose_renaming_open_right n (r : renaming term) :=
-    match r with
-    | r_id => r
-    | r_shift n2 r =>
-      r_shift
-        (transpose_open_pop_right
-           (transpose_opens_renaming_open_left nil r n) n2)
-        (transpose_renaming_open_right n r)
-    | r_rename n2 r n3 =>
-      if name_dec n n3 then r
-      else
-        r_rename
-          (transpose_open_pop_right
-             (transpose_opens_renaming_open_left
-                nil r (unshift_name n3 n)) n2)
-          (transpose_renaming_open_right (unshift_name n3 n) r)
-          (unshift_name n n3)
-    | r_subst t r n2 =>
-      if name_dec n n2 then r
-      else
-        r_subst
-          t (transpose_renaming_open_right (unshift_name n2 n) r)
-          (unshift_name n n2)
-    end.
-  Arguments transpose_renaming_open_right n r
-    : simpl nomatch.
-
-  Fixpoint compose_renaming
-           (r1 : renaming term) (r2 : renaming term) :=
-    match r2 with
-    | r_id => r1
-    | r_shift n r2 =>
-      match transpose_opens_renaming_open_left nil r1 n with
-      | p_open n' =>
-        r_shift n'
-          (compose_renaming (transpose_renaming_open_right n r1) r2)
-      | p_bind _ =>
-          compose_renaming (transpose_renaming_open_right n r1) r2
-      end
-    | r_rename n1 r2 n2 =>
-      match transpose_opens_renaming_open_left nil r1 n1 with
-      | p_open n1' =>
-        r_rename n1'
-          (compose_renaming (transpose_renaming_open_right n1 r1) r2) n2
-      | p_bind t =>
-        r_subst t
-          (compose_renaming (transpose_renaming_open_right n1 r1) r2) n2
-      end
-    | r_subst t r2 n =>
-      r_subst (apply_renaming r1 t) (compose_renaming r1 r2) n
-    end.
-  Arguments compose_renaming r1 r2 : simpl nomatch.
-
-  Notation "r1 @ r2" := (compose_renaming r1 r2) : ren_scope.
-
-  (* Reductions *)
-
-  Lemma red_transpose_opens_renaming_open_left_rename_eq
-        ns n1 r n2 n3 :
-    n2 = n3 ->
-    transpose_opens_renaming_open_left ns (r_rename n1 r n2) n3
-    = p_open (transpose_opens_open_left ns n1).
-  Proof.
-    unfold transpose_opens_renaming_open_left.
-    fold transpose_opens_renaming_open_left.
-    destruct (name_dec n3 n2); congruence.
-  Qed.
-
-  Lemma red_transpose_opens_renaming_open_left_rename_neq
-        ns n1 r n2 n3 :
-    n2 <> n3 ->
-    transpose_opens_renaming_open_left ns (r_rename n1 r n2) n3
-    = transpose_opens_renaming_open_left
-        (cons n1 ns) r (unshift_name n2 n3).
-  Proof.
-    unfold transpose_opens_renaming_open_left.
-    fold transpose_opens_renaming_open_left.
-    destruct (name_dec n3 n2); congruence.
-  Qed.
-
-  Lemma red_transpose_opens_renaming_open_left_subst_eq
-        ns t r n1 n2 :
-    n1 = n2 ->
-    transpose_opens_renaming_open_left ns (r_subst t r n1) n2
-    = p_bind (transpose_opens_bind_left ns t).
-  Proof.
-    unfold transpose_opens_renaming_open_left.
-    fold transpose_opens_renaming_open_left.
-    destruct (name_dec n2 n1); congruence.
-  Qed.
-
-  Lemma red_transpose_opens_renaming_open_left_subst_neq
-        ns t r n1 n2 :
-    n1 <> n2 ->
-    transpose_opens_renaming_open_left ns (r_subst t r n1) n2
-    = transpose_opens_renaming_open_left ns r (unshift_name n1 n2).
-  Proof.
-    unfold transpose_opens_renaming_open_left.
-    fold transpose_opens_renaming_open_left.
-    destruct (name_dec n2 n1); congruence.
-  Qed.
-
-  Lemma red_transpose_renaming_open_right_rename_eq
-    n1 n2 r n3 :
-    n1 = n3 ->
-    transpose_renaming_open_right n1 (r_rename n2 r n3) = r.
-  Proof.
-    unfold transpose_renaming_open_right.
-    fold transpose_renaming_open_right.
-    destruct (name_dec n1 n3); congruence.
-  Qed.
-
-  Lemma red_transpose_renaming_open_right_rename_neq
-    n1 n2 r n3 :
-    n1 <> n3 ->
-    transpose_renaming_open_right n1 (r_rename n2 r n3)
-    = r_rename
-        (transpose_open_pop_right
-           (transpose_opens_renaming_open_left
-              nil r (unshift_name n3 n1)) n2)
-        (transpose_renaming_open_right (unshift_name n3 n1) r)
-        (unshift_name n1 n3).
-  Proof.
-    unfold transpose_renaming_open_right.
-    fold transpose_renaming_open_right.
-    destruct (name_dec n1 n3); congruence.
-  Qed.
-
-  Lemma red_transpose_renaming_open_right_subst_eq
-        n1 t r n2 :
-    n1 = n2 ->
-    transpose_renaming_open_right n1 (r_subst t r n2) = r.
-  Proof.
-    unfold transpose_renaming_open_right.
-    fold transpose_renaming_open_right.
-    destruct (name_dec n1 n2); congruence.
-  Qed.
-
-  Lemma red_transpose_renaming_open_right_subst_neq
-        n1 t r n2 :
-    n1 <> n2 ->
-    transpose_renaming_open_right n1 (r_subst t r n2)
-    = r_subst t
-        (transpose_renaming_open_right (unshift_name n2 n1) r)
-        (unshift_name n1 n2).
-  Proof.
-    unfold transpose_renaming_open_right.
-    fold transpose_renaming_open_right.
-    destruct (name_dec n1 n2); congruence.
-  Qed.
-
-  Lemma red_compose_renaming_shift r1 n r2 :
-    compose_renaming r1 (r_shift n r2)
-    = r_pop_weak
-        (transpose_opens_renaming_open_left nil r1 n)
-        (compose_renaming (transpose_renaming_open_right n r1) r2).
-  Proof. easy. Qed.
-
-  Lemma red_compose_renaming_rename r1 n1 r2 n2 :
-    compose_renaming r1 (r_rename n1 r2 n2)
-    = r_pop_close
-        (transpose_opens_renaming_open_left nil r1 n1)
-        (compose_renaming (transpose_renaming_open_right n1 r1) r2)
-        n2.
-  Proof. easy. Qed.
-
-  Hint Rewrite red_transpose_opens_renaming_open_left_rename_eq
-       red_transpose_opens_renaming_open_left_rename_neq
-       red_transpose_opens_renaming_open_left_subst_eq
-       red_transpose_opens_renaming_open_left_subst_neq
-       red_transpose_renaming_open_right_rename_eq
-       red_transpose_renaming_open_right_rename_neq
-       red_transpose_renaming_open_right_subst_eq
-       red_transpose_renaming_open_right_subst_neq
-    using (cbn; congruence) : reduce_renamings.
-
-  Hint Rewrite red_compose_renaming_shift
-       red_compose_renaming_rename : reduce_renamings.
-
-  Ltac reduce_renamings :=
-    autorewrite with reduce_renamings;
-    repeat progress
-      (try (rewrite_strat topdown (hints reduce_renamings)); cbn).
-
-  (* Represent operations using the [ivar] primitives. *)
-  Module AsIVars.
-
-    Lemma open_k_def n :
-      @open_k n =m= open_ivar n (@unit 0).
-    Proof.
-      rewrite open_ivar_as_composition.
-      unfold open_k; autorewrite with var_ops_as_ivars.
-      easy.
-    Qed.
-
-    Lemma close_k_def n :
-      @close_k n =m= close_ivar n (@unit 1).
-    Proof.
-      rewrite close_ivar_as_composition.
-      unfold close_k; autorewrite with var_ops_as_ivars.
-      easy.
-    Qed.
-
-    Lemma weak_k_def :
-      @weak_k =m= weak_ivar (@unit 1).
-    Proof.
-      rewrite weak_ivar_as_composition.
-      easy.
-    Qed.
-
-    Lemma bind_k_def t :
-      @bind_k t = bind_ivar (@weaken t) (@unit 0).
-    Proof. easy. Qed.
-
-    Lemma open_def n :
-      @open n =m= kleisli (open_ivar n (@unit 0)).
-    Proof.
-      unfold open; rewrite open_k_def; easy.
-    Qed.
-
-    Lemma close_def n :
-      @close n =m= kleisli (close_ivar n (@unit 1)).
-    Proof.
-      unfold close; rewrite close_k_def; easy.
-    Qed.
-
-    Lemma weak_def :
-      @weak =m= kleisli (weak_ivar (@unit 1)).
-    Proof.
-      unfold weak; rewrite weak_k_def; easy.
-    Qed.
-
-    Lemma bind_def t :
-    @bind t = kleisli (bind_ivar (@weaken t) (@unit 0)).
-    Proof. easy. Qed.
-
-    Lemma apply_renaming_k_id_def :
-      @apply_renaming_k r_id =m= @unit 0.
-    Proof. easy. Qed.
-
-    Lemma apply_renaming_k_shift_def n r :
-      @apply_renaming_k (r_shift n r)
-      =m= kleisli (open_ivar n (@unit 0))
-          @ morph_extend (@apply_renaming_k r)
-          @ IVar.weak_var.
-    Proof.
-      intros V v; cbn.
-      unfold apply_renaming_k; fold apply_renaming_k.
-      destruct (reducible (r_shift n r) v).
-      rewrite open_def, weak_var_def.
-      easy.
-    Qed.
-
-    Lemma apply_renaming_k_rename_def n1 r n2 :
-      @apply_renaming_k (r_rename n1 r n2)
-      =m= kleisli (open_ivar n1 (@unit 0))
-          @ morph_extend (@apply_renaming_k r)
-          @ IVar.close_var n2.
-    Proof.
-      intros V v; cbn.
-      unfold apply_renaming_k; fold apply_renaming_k.
-      destruct (reducible (r_rename n1 r n2) v).
-      rewrite open_def, close_var_def.
-      easy.
-    Qed.
-
-    Lemma apply_renaming_k_subst_def t r n :
-      @apply_renaming_k (r_subst t r n)
-      =m= kleisli (bind_ivar (@weaken t) (@unit 0))
-          @ morph_extend (@apply_renaming_k r)
-          @ IVar.close_var n.
-    Proof.
-      intros V v; cbn.
-      unfold apply_renaming_k; fold apply_renaming_k.
-      destruct (reducible (r_subst t r n) v).
-      rewrite bind_def, close_var_def.
-      easy.
-    Qed.
-
-    Lemma apply_renaming_id_def :
-      @apply_renaming r_id =m= 1.
-    Proof.
-      unfold apply_renaming.
-      rewrite apply_renaming_k_id_def, right_identity.
-      easy.
-    Qed.
-
-    Lemma apply_renaming_shift_def n r :
-      @apply_renaming (r_shift n r)
-      =m= kleisli (open_ivar n (@unit 0))
-          @ kleisli (morph_extend (@apply_renaming_k r))
-          @ kleisli (weak_ivar (@unit 1)).
-    Proof.
-      unfold apply_renaming.
-      rewrite apply_renaming_k_shift_def,
-        !associativity, weak_ivar_as_composition,
-        morph_associative with (g := @unit 1), left_identity.
-      easy.
-    Qed.
-
-    Lemma apply_renaming_rename_def n1 r n2 :
-      @apply_renaming (r_rename n1 r n2)
-      =m= kleisli (open_ivar n1 (@unit 0))
-          @ kleisli (morph_extend (@apply_renaming_k r))
-          @ kleisli (close_ivar n2 (@unit 1)).
-    Proof.
-      unfold apply_renaming.
-      rewrite apply_renaming_k_rename_def,
-        !associativity, close_ivar_as_composition,
-        morph_associative with (g := @unit 1), left_identity.
-      easy.
-    Qed.
-
-    Lemma apply_renaming_subst_def t r n :
-      @apply_renaming (r_subst t r n)
-      =m= kleisli (bind_ivar (@weaken t) (@unit 0))
-          @ kleisli (morph_extend (@apply_renaming_k r))
-          @ kleisli (close_ivar n (@unit 1)).
-    Proof.
-      unfold apply_renaming.
-      rewrite apply_renaming_k_subst_def,
-        !associativity, close_ivar_as_composition,
-        morph_associative with (g := @unit 1), left_identity.
-      easy.
-    Qed.
-
-    Hint Rewrite open_k_def close_k_def weak_k_def bind_k_def
-         open_def close_def weak_def bind_def
-         apply_renaming_k_id_def
-         apply_renaming_k_shift_def
-         apply_renaming_k_rename_def
-         apply_renaming_k_subst_def
-         apply_renaming_id_def
-         apply_renaming_shift_def
-         apply_renaming_rename_def
-         apply_renaming_subst_def
-      : term_ops_as_ivars.
-
-    Lemma weaken_extend t :
-      pnset_extend (@weaken t)
-      =p= morph_apply
-            (kleisli (weak_ivar (@unit 1)))
-            (@weaken t).
-    Proof.
-      intro V; cbn; autorewrite with term_ops_as_ivars; easy.
-    Qed.
-
-    Hint Rewrite @left_identity @right_identity
-         @associativity @unit_extend @kleisli_extend
-         @weaken_extend
-         @morph_apply_compose @morph_apply_id
-         @pair_ivar_compose_distribute
-         @fst_ivar_compose_distribute
-         @snd_ivar_compose_distribute
-         @open_ivar_compose_distribute
-         @close_ivar_compose_distribute
-         @weak_ivar_compose_distribute
-         @bind_ivar_compose_distribute
-         @swap_ivar_compose_distribute
-         @pair_ivar_extend @fst_ivar_extend
-         @snd_ivar_extend @open_ivar_extend
-         @close_ivar_extend @weak_ivar_extend
-         @bind_ivar_extend @swap_ivar_extend
-      : simpl_terms_as_ivars.
-
-    Hint Rewrite <- @open_ivar_as_composition
-        @close_ivar_as_composition @weak_ivar_as_composition
-      : simpl_terms_as_ivars.
-
-    Ltac simpl_terms_as_ivars :=
-      autorewrite with var_ops_as_ivars term_ops_as_ivars;
-      autorewrite with simpl_terms_as_ivars;
-      repeat progress
-        (cbn;
-         try (rewrite_strat topdown
-                (hints simpl_terms_as_ivars))).
-
-    Lemma snd_ivar_apply_renaming_k r :
-      snd_ivar (@apply_renaming_k r)
-      =m= snd_ivar (@unit 0).
-    Proof.
-      induction r; simpl_terms_as_ivars.
-      - easy.
-      - rewrite <- ivar_eta with (f := @apply_renaming_k r).
-        rewrite IHr.
-        simpl_terms_as_ivars; simpl_ivars; easy.
-      - rewrite <- ivar_eta with (f := @apply_renaming_k r).
-        rewrite IHr.
-        simpl_terms_as_ivars; simpl_ivars; easy.
-      - rewrite <- ivar_eta with (f := @apply_renaming_k r).
-        rewrite IHr.
-        simpl_terms_as_ivars; simpl_ivars; easy.
-    Qed.
-
-    Lemma apply_renaming_k_pair_eta r :
-      @apply_renaming_k r
-      =m= pair_ivar (fst_ivar (@apply_renaming_k r))
-                    (snd_ivar (@unit 0)).
-    Proof.
-      rewrite <- snd_ivar_apply_renaming_k.
-      simpl_ivars; easy.
-    Qed.
-
-  End AsIVars.
-
-  Import AsIVars.
-
-  (* Normalization *)
-
-  Lemma combine_open_renaming_close N n1 r n2 (t : term N):
-    open n1 ([r](close n2 t))
-    = [r; n1 <- n2] t.
-  Proof.
-    unfold open, close, apply_renaming at 1.
-    simpl_terms_as_ivars.
-Qed.
-
-  Lemma combine_open_renaming_weak N n r (t : term N) :
-    open n ([r](weak t))
-    = [r; ^n] t.
-  Proof. easy. Qed.
-
-  Lemma combine_bind_renaming_close N t1 r n (t2 : term N) :
-    bind t1 ([r](close n t2))
-    = [r; t1 // n] t2.
-  Proof. easy. Qed.
-
-  Lemma combine_bind_renaming_weak N t1 r (t2 : term N) :
-    bind t1 ([r](weak t2))
-    = [r] t2.
-  Proof.
-    simpl_terms_as_ivars.
-    
-
-  (* Simplification *)
-
-
-  Lemma transpose_open_pop n p :
-    @open n @ morph_extend (apply_pop p)
-    =m= apply_pop (transpose_open_pop_left n p)
-        @ morph_extend (@open (transpose_open_pop_right p n)).
-  Proof.
-    destruct p; cbn.
-    - simpl_terms_as_ivars.
-      transpose_ivar_pop_pop (open _) (open _).
-    autorewrite with unfold_terms.
-    autorewrite with simpl_terms.
-    transpose_ivar_pop_pop (open n0) (open n).
-
-Definition apply_pop (op : pop term)
-  : morph term 1 term 0 :=
-  match op with
-  | p_open n => @open n
-  | p_bind t => @bind t
-  end.
-Arguments apply_pop !op.
-
-Definition transpose_renaming_bind (r : renaming term) t :
-  pop term * renaming term :=
-  pair (p_bind (apply_renaming r 0 t)) r.
-
-Definition transpose_renaming_pop (r : renaming term) p :
-  pop term * renaming term :=
-  match p with
-  | p_open n => transpose_renaming_open r n
-  | p_bind t => transpose_renaming_bind r t
-  end.
-
-Lemma snd_apply_static_ivar {N T M} (r : renaming T)
-      (f : ivar N T M) :
-  snd_ivar (apply_static_ivar r f) = snd_ivar f.
-Proof.
-  generalize dependent M.
-  generalize dependent N.
-  induction r; intros N M f; cbn.
-  - easy.
-  - simpl_ivars_pointwise.
-    rewrite IHr; easy.
-  - simpl_ivars_pointwise.
-    rewrite IHr; easy.
-  - easy.
-Qed.
-
-Lemma fst_apply_static_ivar {N T M} (r : renaming T)
-      (f : ivar N T M) (g : ivar N T M) :
-  fst_ivar f =km= fst_ivar g ->
-  fst_ivar (apply_static_ivar r f)
-  =km= fst_ivar (apply_static_ivar r g).
-Proof.
-  generalize dependent M.
-  generalize dependent N.
-  induction r; intros N M f g Heq; cbn.
-  - easy.
-  - simpl_ivars_pointwise.
-    apply IHr.
-    simpl_ivars_pointwise.
-    rewrite Heq; easy.
-  - simpl_ivars_pointwise.
-    rewrite snd_apply_static_ivar, snd_apply_static_ivar.
-    simpl_ivars_pointwise.
-    rewrite Heq.
-    rewrite IHr with (g := open_ivar b g); try easy.
-    simpl_ivars_pointwise.
-    rewrite Heq; easy.
-  - apply IHr; easy.
-Qed.
-
-Lemma transpose_swap_ivar_apply_static_ivar {N T M}
-      (r : renaming T)
-      (f : ivar (S (S N)) T M) :
-  swap_ivar (apply_static_ivar r f)
-  =m= apply_static_ivar r (swap_ivar f).
-Proof.
-  unfold swap_ivar; symmetry.
-  rewrite <- ivar_eta_pointwise.
-  rewrite snd_apply_static_ivar, snd_apply_static_ivar.
-  rewrite fst_apply_static_ivar with (g := f) by easy.
-  simpl_ivars_pointwise.
-  easy.
-Qed.
-
-Lemma transfer_open_var_spec {T} (r : renaming T) n :
-  forall {N M} (f : ivar N T M),
-  open_ivar n (apply_static_ivar r f)
-  =m= apply_static_ivar
-        (snd (transfer_open_var r n))
-        (open_ivar (fst (transfer_open_var r n)) f).
-Proof.
-  generalize dependent n.
-  induction r; intros c N M f; cbn in *.
-  - easy.
-  - rewrite transpose_open_ivar_weak_ivar_pointwise.
-    rewrite IHr.
-    rewrite transpose_swap_ivar_apply_static_ivar.
-    rewrite transpose_open_ivar_open_ivar_pointwise.
-    easy.
-  - remember (name_eqb c n) as eq_ca eqn:Hca.
-    symmetry in Hca.
-    destruct eq_ca.
-    + apply name_eqb_eq in Hca; subst.
-      simpl_ivars_pointwise.
-      easy.
-    + apply name_eqb_neq in Hca.
-      rewrite transpose_open_ivar_close_ivar_pointwise
-        by easy.
-      rewrite IHr.
-      rewrite transpose_swap_ivar_apply_static_ivar.
-      rewrite transpose_open_ivar_open_ivar_pointwise.
-      easy.
-  - rewrite IHr.
-    easy.
-Qed.
-
-Lemma compose_static_left_identity {T} (r : renaming T) :
-  compose_static r_id r = r.
-Proof. easy. Qed.
-
-Lemma compose_static_right_identity {T} (r : renaming T) :
-  compose_static r r_id = r.
-Proof.
-  induction r; cbn; try rewrite IHr; easy.
-Qed.
-
-(*
-Lemma transfer_open_var_shift_name {T} (r : renaming T) a b :
-  fst (transfer_open_var r (shift_name a b))
-  = shift_name (fst (transfer_open_var r a))
-      (fst (transfer_open_var (snd (transfer_open_var r a)) b)).
-Proof.
-  generalize dependent b.
-  generalize dependent a.
-  induction r; intros c d; cbn.
-  - easy.
-  - rewrite IHr.
-    rewrite transpose_shift_name_shift_name.
-    easy.
-  - remember (name_eqb c a) as eq_ca eqn:Hca.
-    symmetry in Hca.
-    remember (name_eqb (shift_name c d) a) as eq_da eqn:Hda.
-    symmetry in Hda.
-    destruct eq_ca, eq_da; cbn.
-    + apply name_eqb_eq in Hca.
-      apply name_eqb_eq in Hda; subst.
-      contradict Hda.
-      apply shift_name_neq.
-    + apply name_eqb_eq in Hca; subst.
-      simpl_names; easy.
-    + apply name_eqb_neq in Hca.
-      apply name_eqb_eq in Hda; subst.
-      simpl_names.
-      easy.
-    + apply name_eqb_neq in Hca.
-      apply name_eqb_neq in Hda.
-      remember (name_eqb d (unshift_name c a))
-        as dca eqn:Hdca.
-      symmetry in Hdca.
-      destruct dca.
-      * rewrite name_eqb_eq in Hdca; subst.
-        contradict Hda.
-        simpl_names; easy.
-      * rewrite name_eqb_neq in Hdca.
-        simpl_names; cbn.
-        rewrite <- transpose_shift_name_shift_name.
-        rewrite <- IHr.
-        rewrite transpose_unshift_name_shift_name by easy.
-        easy.
-  - apply IHr.
-Qed.
-
-Lemma transfer_open_var_unshift_name {T} (r : renaming T) a b :
-  fst (transfer_open_var
-         (snd (transfer_open_var r (shift_name a b)))
-         (unshift_name b a))
-  = unshift_name
-      (fst (transfer_open_var (snd (transfer_open_var r a)) b))
-      (fst (transfer_open_var r a)).
-Proof.
-  generalize dependent b.
-  generalize dependent a.
-  induction r; intros c d; cbn.
-  - easy.
-  - rewrite IHr.
-    rewrite transfer_open_var_shift_name.
-    remember (fst
-          (transfer_open_var
-             (snd (transfer_open_var r c)) d)) as e.
-    remember (fst (transfer_open_var r c)) as f.
-    rewrite transpose_shift_name_unshift_name.
-
-    
-
-    easy.
-  - remember (name_eqb c a) as eq_ca eqn:Hca.
-    symmetry in Hca.
-    remember (name_eqb (shift_name c d) a) as eq_da eqn:Hda.
-    symmetry in Hda.
-    destruct eq_ca, eq_da; cbn.
-    + apply name_eqb_eq in Hca.
-      apply name_eqb_eq in Hda; subst.
-      contradict Hda.
-      apply shift_name_neq.
-    + apply name_eqb_eq in Hca; subst.
-      simpl_names; easy.
-    + apply name_eqb_neq in Hca.
-      apply name_eqb_eq in Hda; subst.
-      simpl_names.
-      easy.
-    + apply name_eqb_neq in Hca.
-      apply name_eqb_neq in Hda.
-      remember (name_eqb d (unshift_name c a))
-        as dca eqn:Hdca.
-      symmetry in Hdca.
-      destruct dca.
-      * rewrite name_eqb_eq in Hdca; subst.
-        contradict Hda.
-        simpl_names; easy.
-      * rewrite name_eqb_neq in Hdca.
-        simpl_names; cbn.
-        rewrite <- transpose_shift_name_shift_name.
-        rewrite <- IHr.
-        rewrite transpose_unshift_name_shift_name by easy.
-        easy.
-  - apply IHr.
-
-*)
-Lemma transfer_open_var_compose_static_fst {T}
-      (r s : renaming T) a :
-   fst (transfer_open_var (compose_static r s) a)
-   = fst (transfer_open_var s (fst (transfer_open_var r a))).
-Proof.
-  generalize dependent a.
-  generalize dependent s.
-  induction r; intros s c; cbn.
-  - easy.
-  - rewrite IHr.
-    rewrite transfer_open_var_open_var.
-    easy.
-  - remember (name_eqb c a) as ca eqn:Hca.
-    symmetry in Hca.
-    destruct ca.
-    + rewrite name_eqb_eq in Hca; subst.
-      easy.
-    + rewrite IHr.
-      simpl_ivars.
-      rewrite transfer_open_var_open_var.
-      easy.
-  - apply IHr.
-Qed.
-
-Lemma transfer_open_var_compose_static_snd {T}
-      (r s : renaming T) a :
-  snd (transfer_open_var (compose_static r s) a)
-  = compose_static (snd (transfer_open_var r a))
-      (snd (transfer_open_var s (fst (transfer_open_var r a)))).
-Proof.
-  generalize dependent a.
-  generalize dependent s.
-  induction r; intros s c; cbn.
-  - easy.
-  - f_equal.
-    + rewrite transfer_open_var_compose_static_fst.
-    rewrite IHr.
-    
-    easy.
-  - remember (name_eqb c a) as ca eqn:Hca.
-    symmetry in Hca.
-    destruct ca.
-    + rewrite name_eqb_eq in Hca; subst.
-      easy.
-    + rewrite IHr.
-      simpl_ivars.
-      rewrite transfer_open_var_open_var.
-      easy.
-  - apply IHr.
-Qed.
-
-Lemma compose_static_associative {T} (r s t : renaming T) :
-  compose_static r (compose_static s t)
-  = compose_static (compose_static r s) t.
-Proof.
-  generalize dependent s.
-  generalize dependent t.
-  induction r; intros u s; cbn.
-  - easy.
-  - rewrite transfer_open_var_compose_static.
-    rewrite <- IHr.
-    f_equal.
-  -
-  - rewrite IHr; easy.
-Qed.
-
-Lemma apply_static_ivar_compose {T N T M} (r : renaming T) s
-      (f : ivar N T M) :
-  apply_static_ivar (compose_static r s) f
-  =m= apply_static_ivar r (apply_static_ivar s f).
-Proof.
-  generalize dependent M.
-  generalize dependent T.
-  generalize dependent N.
-  generalize dependent s.
-  induction r; intros s N T M f; cbn.
-  - easy.
-  - rewrite transfer_open_var_spec by eassumption.
-    rewrite <- IHr.
-    easy.
-  - rewrite transfer_open_var_spec by eassumption.
-    rewrite <- IHr.
-    easy.
-  - easy.
-Qed.
-
-Lemma apply_static_ivar_as_composition {T N T M} (r : renaming T)
-      (f : ivar N T M) :
-  apply_static_ivar r f =m=
-  f @ (morph_extend_by N (apply_static_var r)).
-Proof.
-  generalize dependent M.
-  generalize dependent T.
-  generalize dependent N.
-  induction r; intros N T M f; cbn.
-  - rewrite morph_extend_by_id.
-    easy.
-  - rewrite morph_extend_by_compose, morph_extend_by_compose.
-    rewrite weak_ivar_as_composition, open_ivar_as_composition.
-    rewrite IHr; cbn.
-    easy.
-  - rewrite morph_extend_by_compose, morph_extend_by_compose.
-    rewrite close_ivar_as_composition, open_ivar_as_composition.
-    rewrite IHr.
-    easy.
-  - apply IHr.
-Qed.
-
-Lemma apply_static_var_spec {T} (r : renaming T) :
-  apply_static_var r =m= apply_static_ivar r 1.
-Proof.
-  induction r; cbn.
-  - easy.
-  - rewrite weak_ivar_as_composition, open_ivar_as_composition,
-      apply_static_ivar_as_composition.
-    easy.
-  - rewrite close_ivar_as_composition, open_ivar_as_composition,
-      apply_static_ivar_as_composition.
-    easy.
-  - easy.
-Qed.
-
-Lemma apply_static_ivar_compose_distribute {T N T M R L}
-      (r : renaming T) (f : ivar N T M) (g : morph T M R L) :
-  g @ (apply_static_ivar r f)
-  =m= apply_static_ivar r (g @ f).
-Proof.
-  intros V v.
-  rewrite apply_static_ivar_as_composition.
-  rewrite morph_associative.
-  rewrite <- apply_static_ivar_as_composition.
-  easy.
-Qed.
-
-Lemma apply_static_var_compose {T N T M} (r : renaming T) s
-      (f : ivar N T M) :
-  apply_static_var (compose_static r s)
-  =m= (apply_static_var s) @ (apply_static_var r).
-Proof.
-  rewrite apply_static_var_spec.
-  rewrite apply_static_ivar_compose.
-  rewrite apply_static_ivar_as_composition, apply_static_ivar_as_composition.
-  easy.
-Qed.
-
-End TermLemmas.
+End MakeTerm.
